Generalize step 2, new example and use copy in elpi

theories/refinement_elimination.v
@@ -1,23 +1,41 @@
-From Ltac2 Require Import Ltac2.
+Require Import expand.
+Require Import unfold_reflexivity.
+Require Import unfold_in.
+Require Import reflexivity.
 From elpi Require Import elpi.
+From Ltac2 Require Import Ltac2.
+From Ltac2 Require Import Printf.
+Import Constr.Unsafe.
+
 
 Set Default Proof Mode "Classic".
 
-Require Import refinement_elimination_elpi.
 
-Definition p (n : nat) : Prop := n >= 3.
 
-Definition t := { x : nat | p x }.
+(* Definition p (n : nat) : Prop := n >= 3. *)
 
-Definition x : t := exist _ 3 (le_n 3).
+(* Definition t := { x : nat | p x }. *)
 
-Tactic Notation "step_one" ident(i) constr(x) :=
-  elpi step_one_tac ltac_string:(i) ltac_term:(x).
+(* Definition x : t := exist _ 3 (le_n 3). *)
 
-Goal (proj1_sig x) >= 3.
-  step_one foo (exist p 3 (le_n 3)).
-  Abort.
 
+(* Definition identity {A : Type} : A -> A := fun x => x. *)
+
+(* Goal (proj1_sig x) >= 3. *)
+(*   step_one foo (exist p 3 (le_n 3)). *)
+(*   pose (y := exist p 3 (le_n 3)). *)
+(*   step_one foo2 y. *)
+(*   step_one bar (fun x : @sig nat p => exist p (proj1_sig x) (proj2_sig x)). *)
+(*   step_one baz (let z : @sig nat p := exist p 3 (le_n 3) in z). *)
+
+(*   step_one baz2 ((fun k : @sig nat p -> @sig nat p => k y) id). *)
+(*   (* This one does not work *) *)
+
+
+(*   step_one baz3 (fun k : @sig nat p -> @sig nat p => k y). *)
+(*   Abort. *)
+
+(* The trigger should be activated for any symbol that contains a refinement type in its type *)
 (* param p: symbol whose type contain a refinement type *)
 (* 1. Define new equivalent symbol free of refinement types *)
 (* 2. Prove that the first projection of p is equal to the new symbol *)
@@ -27,44 +45,227 @@ Goal (proj1_sig x) >= 3.
 Ltac2 fail msg :=
   Control.zero (Tactic_failure (Some msg)).
 
-Ltac2 get_pred (tp:constr) : constr :=
-  lazy_match! tp with
-    | @sig _ ?pa => pa
-    | _ => fail (Message.concat (Message.of_string "Expected refinement type but got: ") (Message.of_constr tp))
+Ltac2 rec make_eq' (f : constr) (g : constr) (gA : constr) (gP : constr) (t : constr) (i : int) (args : constr list) :=
+  match kind t with
+  | Prod b c =>
+      make (Prod b (make_eq' f g gA gP c (Int.add i 1) (make (Rel i) :: args)))
+  | _ =>
+      let lhs := make (App f (Array.of_list args)) in
+      let rhs := make (App g (Array.of_list args)) in
+      let rhs' := make (App constr:(proj1_sig) (Array.of_list [gA; gP; rhs])) in
+      make (App constr:(@eq) (Array.of_list [t; lhs; rhs']))
   end.
 
-(*Definition get_pred {A : Type} {P : A -> Prop} : @sig A P -> (A -> Prop) := fun _ => P.*)
+Ltac2 rec get_ret_sig (t : constr) : constr * constr :=
+  match kind t with
+    | Prod _ c => get_ret_sig c
+    | _ =>
+       lazy_match! t with
+         | @sig ?d ?p => (d, p)
+         | _ => fail (Message.concat (Message.of_string "Expected refinement type but got: ") (Message.of_constr t))
+       end
+  end.
 
-Ltac elim_refinement_types foo p :=
+Ltac2 make_eq (f : constr) (g : constr) (reducedTypeG : constr) :=
+  let (gA, gP) := get_ret_sig reducedTypeG in
+  make_eq' f g gA gP (Constr.type f) 1 [].
+
+Ltac2 rec make_pred' (f : constr) (tF : constr) (pred : constr) (i : int) (args : constr list) :=
+  match kind tF with
+  | Prod b c =>
+      make (Prod b (make_pred' f c pred (Int.add i 1) (make (Rel i) :: args)))
+  | _ =>
+      let fApplied := make (App f (Array.of_list args)) in
+      make (App pred (Array.of_list [fApplied]))
+  end.
+
+Ltac2 make_pred (f : constr) (pred : constr) :=
+  make_pred' f (Constr.type f) pred 1 [].
+
+
+Require Import refinement_elimination_elpi.
+
+Tactic Notation "step_one" ident(i) constr(x) :=
+  elpi step_one_tac ltac_string:(i) ltac_term:(x).
+
+Ltac elim_refinement_types p :=
   (* Step 1 *)
+  let f1 := fresh "step_one" in
   let p2 := eval hnf in p in
-  step_one foo p;
+  step_one f1 p2;
 
   (* Step 2 *)
-  let pf_refl := fresh "pf_refl" in
-  assert (pf_refl : proj1_sig p = foo) by reflexivity;
-
-  (* Step 3 *)
+  let f1 := eval cbn in f1 in
+  let pf_refl := fresh "step_two" in
   let tp := type of p in
-  let tp := eval hnf in tp in
-  let tac :=
-    ltac2:(new_p_id' tp' pf_refl' |-
-      let pred := Ltac1.of_constr (get_pred (Option.get (Ltac1.to_constr tp'))) in
-      (* TODO: We really just want to beta reduce one time, maybe head normal form is too strong *)
-      ltac1:(pred' new_p_id'' pf_refl'' |- let pred_applied := constr:(pred' new_p_id'') in let pred_applied := (eval hnf in pred_applied) in assert (pred_applied) by (rewrite <- pf_refl''; apply proj2_sig)) pred new_p_id' pf_refl'
-    )
-  in tac foo tp pf_refl;
+  let tp := eval red in tp in
+  let tac := ltac2:(f1' p' redPType pf_refl |-
+    let f1'' := Option.get (Ltac1.to_constr f1') in
+    let p'' := Option.get (Ltac1.to_constr p') in
+    let redPType' := Option.get (Ltac1.to_constr redPType) in
+    let eq := make_eq f1'' p'' redPType' in
+    ltac1:(eq' pf_refl' |- assert (pf_refl' : eq') by now simpl) (Ltac1.of_constr eq) pf_refl
+  ) in tac f1 p tp pf_refl.
 
-  (* Step 4 *)
-  rewrite pf_refl in *;
+  (* (* Step 3 *) *)
+  (* let tac := ltac2:(f1' tp' pf_refl' |- *)
+  (*     let tp'2 := Option.get (Ltac1.to_constr tp') in *)
+  (*     let (_, pred) := get_ret_sig tp'2 in *)
+  (*     (* let pred := Ltac1.of_constr pred' in *) *)
+  (*     let pred_applied := make_pred (Option.get (Ltac1.to_constr f1')) pred in *)
+  (* (*     (* TODO: We really just want to beta reduce one time, maybe head normal form is too strong, maybe a bit of ELPI here would help *) *) *)
+  (*     ltac1:(pred' f1'' pf_refl'' |- *)
+  (*       (* let pred' := eval cbn in pred' in *) *)
+  (*       assert (pred') by (intros; rewrite pf_refl''; apply proj2_sig) *)
+  (*     ) (Ltac1.of_constr pred_applied) f1' pf_refl' *)
+  (*   ) *)
+  (* in tac f1 tp pf_refl. *)
 
-  clear pf_refl.
 
-Goal (proj1_sig (exist p 3 (le_n 3))) >= 3.
-  (* assert (H:x = exist _ 3 (le_n 3)) by reflexivity. *)
-  elim_refinement_types foo (exist p 3 (le_n 3)).
+  (* (* (* Step 4 *) *) *)
+  (* rewrite pf_refl in *; *)
 
-  Goal forall (x : t) , (proj1_sig x) >= 3.
-  intro x.
-  elim_refinement_types x.
-  Focus 2.
+  (* clear pf_refl. *)
+
+
+Definition P : nat -> Prop := fun x => x >= 3.
+
+Definition tt := {x : nat | P x}.
+
+Definition v : tt := exist P 3 (le_n 3).
+
+Goal proj1_sig v - 1 >= 2.
+  let f1 := fresh "step_one" in
+  let p2 := eval hnf in v in
+  step_one f1 p2.
+  elim_refinement_types v.
+
+Require Import ZArith.
+
+Open Scope Z.
+
+Inductive data : Type := Nil | Cons (lo hi: Z) (tl: data).
+
+Fixpoint In (x: Z) (s: data) :=
+  match s with
+  | Nil => False
+  | Cons l h s' => l <= x < h \/ In x s'
+  end.
+
+Fixpoint InBool (x: Z) (s: data) : bool :=
+  match s with
+  | Nil => false
+  | Cons l h s' => ((Z.leb l x) && (Z.ltb x h)) || InBool x s'
+  end.
+
+
+Inductive ok: data -> Prop :=
+  | ok_nil: ok Nil
+  | ok_cons: forall l h s
+      (BOUNDS: l < h)
+      (BELOW: forall x, In x s -> h < x)
+      (OK: ok s),
+      ok (Cons l h s).
+
+Fixpoint ok' (x : data) : bool :=
+  match x with
+    | Nil => true
+    | Cons l1 h1 s =>
+        match s with
+        | Nil => l1 <? h1
+        | Cons l2 _ _ => (l1 <? h1) && (h1 <? l2) && (ok' s)
+        end
+  end.
+
+Check @sig.
+
+Definition refData := @sig data (fun r => ok r).
+
+(* Definition refData := { r : data | ok r }. *)
+
+Axiom foo : forall l h , ok (if l <? h then Cons l h Nil else Nil).
+
+Program Definition interval (l h: Z) : refData :=
+  exist _ (if Z.ltb l h then Cons l h Nil else Nil) _.
+Next Obligation.
+  exact (foo l h).
+Defined.
+
+Program Definition InBoolRef (x : Z) (s : refData) : bool := InBool x s.
+
+Theorem In_interval: forall x l h, (InBoolRef x (interval l h) = true) <-> l <= x < h.
+  Proof.
+  split.
+  intro H.
+
+
+  let f1 := fresh "step_one" in
+  let p2 := eval hnf in InBoolRef in
+  step_one f1 p2.
+
+  let f1 := eval cbn in step_one in
+  let tp := type of InBoolRef in idtac tp.
+  let tp := type of InBoolRef in
+  let tp := eval hnf in tp in idtac tp.
+
+  (* Step 2 *)
+  let f1 := eval cbn in f1 in
+  let pf_refl := fresh "step_two" in
+  let tp := type of p in
+  let tp := eval red in tp in
+  let tac := ltac2:(f1' p' redPType pf_refl |-
+    let f1'' := Option.get (Ltac1.to_constr f1') in
+    let p'' := Option.get (Ltac1.to_constr p') in
+    let redPType' := Option.get (Ltac1.to_constr redPType) in
+    let eq := make_eq f1'' p'' redPType' in
+    ltac1:(eq' pf_refl' |- assert (pf_refl' : eq') by now simpl) (Ltac1.of_constr eq) pf_refl
+  ) in tac f1 p tp pf_refl.
+
+
+
+
+
+
+
+  (* let f1 := fresh "step_one" in *)
+  (* let p2 := eval hnf in interval in *)
+  (* step_one f1 p2. *)
+
+  (* let tp := type of interval in *)
+  (* let tp := eval red in tp in *)
+  (* let pf_refl := fresh "step_two" in *)
+  (* let tac := ltac2:(f1' p' redPType pf_refl |- *)
+  (*   let f1'' := Option.get (Ltac1.to_constr f1') in *)
+  (*   let p'' := Option.get (Ltac1.to_constr p') in *)
+  (*   let redPType' := Option.get (Ltac1.to_constr redPType) in *)
+  (*   let eq := make_eq f1'' p'' redPType' in *)
+  (*   ltac1:(eq' pf_refl' |- assert (pf_refl' : eq') by now simpl) (Ltac1.of_constr eq) pf_refl *)
+  (* ) in tac step_one interval tp pf_refl. *)
+
+
+
+  (* let tac := ltac2:(f1' tp' pf_refl' |- *)
+  (*     let tp'2 := Option.get (Ltac1.to_constr tp') in *)
+  (*     let (_, pred) := get_ret_sig tp'2 in *)
+  (*     let pred_applied := make_pred (Option.get (Ltac1.to_constr f1')) pred in *)
+  (* (* (*     (* TODO: We really just want to beta reduce one time, maybe head normal form is too strong, maybe a bit of ELPI here would help *) *) *) *)
+  (*     ltac1:(pred' f1'' pf_refl'' |- *)
+  (*       idtac pred') *)
+  (*       (* let pred' := eval cbn in pred' in *) *)
+  (*       (* assert (pred') (*by (rewrite <- pf_refl''; apply proj2_sig)*)) *) (Ltac1.of_constr pred_applied) f1' pf_refl' *)
+  (*   ) *)
+  (* in tac step_one tp step_two. *)
+  (* intros l h. *)
+  (* rewrite (step_two l h). *)
+
+
+  (* elim_refinement_types interval. *)
+
+  (* intros x0 l h. *)
+  (* split. *)
+  (* intro H. *)
+  (* elim_refinement_types fresh_2 interval. *)
+  (* assert (pf_refl : forall l h , fresh_2 l h = proj1_sig (interval l h)) by reflexivity. *)
+
+  (* elim_refinement_types fresh_1 InBoolRef. *)
+  (* assert (pf_refl : fresh_1 = proj1_sig InBoolRef). *)
