theories/refinement_elimination_elpi.v
@@ -3,20 +3,74 @@ From elpi Require Import elpi.
 Elpi Tactic step_one_tac.
 
 Elpi Accumulate lp:{{
+  shorten std.{map}.
 
-  %copy ({{ exist _ lp:P _ }}) P.
+  pred replace i:term o:term.
+  replace I O :-
+    (copy ({{ exist _ lp:P _ }}) P' :- !, replace P P') =>
+    (copy ({{ @sig lp:A _ }}) A' :- !, replace A A') =>
+    (copy ({{ @proj1_sig _ _ lp:X }}) X' :- !, replace X X') =>
+      copy I O.
 
-  pred step_one i:term, o:term.
-  step_one I O :- (copy ( {{ exist _ lp:P _ }} ) P :- !) => copy I O.
+
+%  pred replace i:term, o:term.
+%  replace I O :-
+%            (copy ({{ exist _ lp:P _ }}) P' :- !, replace P P') =>
+%            (copy ({{ @sig lp:A _ }}) A' :- !, replace A A') =>
+%            (copy ({{ @proj1_sig _ _ lp:X }}) X' :- !, replace X X') =>
+%              copy I O.
+
+%  replace T T' :-
+%            coq.unify-leq T ({{ exist _ lp:P _ }}) ok, !, replace P T'.
+%  replace T T' :-
+%            coq.unify-leq T ({{ @sig lp:A _ }}) ok, !, replace A T'.
+%  replace T T' :-
+%            coq.unify-leq T ({{ @proj1_sig _ _ lp:X }}) ok, !, replace X T'.
+%  replace X Y :- name X, !, X = Y, !. % avoid loading "replace x x" at binders
+%  replace (global _ as C) C :- !.
+%  replace (pglobal _ _ as C) C :- !.
+%  replace (sort _ as C) C :- !.
+%  replace (fun N T F) (fun N T1 F1) :- !,
+%    replace T T1, pi x\ decl x _ T => pi x1\ decl x1 _ T1 => replace x x1 => replace (F x) (F1 x1).
+%  replace (let N T B F) (let N T1 B1 F1) :- !,
+%    replace T T1, replace B B1, pi x\ decl x _ T => pi x1\ decl x1 _ T1 => replace x x1 => replace (F x) (F1 x1).
+%  replace (prod N T F) (prod N T1 F1) :- !,
+%    replace T T1, (pi x\ decl x _ T => pi x1\ decl x1 _ T1 => replace x x1 => replace (F x) (F1 x1)).
+%  replace (app L) (app L1) :- !, map L replace L1.
+%  replace (fix N Rno Ty F) (fix N Rno Ty1 F1) :- !,
+%    replace Ty Ty1, pi x\ decl x _ Ty => pi x1\ decl x1 _ Ty1 => replace x x1 => replace (F x) (F1 x1).
+%  replace (match T Rty B) (match T1 Rty1 B1) :- !,
+%    replace T T1, replace Rty Rty1, map B replace B1.
+%  replace (primitive _ as C) C :- !.
+%  replace (uvar M L as X) W :- var X, !, map L replace L1, coq.mk-app-uvar M L1 W.
+%  % when used in CHR rules
+%  replace (uvar X L) (uvar X L1) :- map L replace L1.
+
+
+%  pred step_one'' i:term, o:term.
+%  step_one'' I O :-
+%      coq.say "step_one'' before: I = " I " | O = " O,
+%      (copy ( {{ exist _ lp:P _ }} ) P :- !) => copy I O,
+%      coq.say "step_one'' after: I = " I " | O = " O.
+%
+%  pred step_one' i:term o:term.
+%  step_one' I O :-
+%      coq.say "step_one' before: I = " I " | O = " O,
+%      (step_one'' ( {{ @sig lp:A _  }} ) A :- !) => step_one'' I O,
+%      coq.say "step_one' after: I = " I " | O = " O.
+%
+%  pred step_one i:term o:term.
+%  step_one I O :-
+%      coq.say "step_one before: I = " I " | O = " O,
+%      (step_one' ( {{ proj1_sig lp:X }} ) X :- !) => step_one' I O,
+%      coq.say "step_one after: I = " I " | O = " O.
 
   solve (goal _ _ _ _ [str S, trm P] as G) GL :-
       !,
       coq.string->name S N,
-      step_one P P',
-      coq.term->string P PS,
-      %coq.say "P:" PS,
-      coq.term->string P' PS2,
-      %coq.say "P':" PS2,
+      replace P P',
+      coq.say "input of replace: " P,
+      coq.say "replace computed: " P',
 
       refine (let N _ P' Tgt_) G GL.
 
